Add Hint Mode to Class ReSum (-<)

secure_example/LabelledImpInline2AsmCorrectness.v
@@ -417,9 +417,11 @@ Section Linking.
 
   Import KTreeFin.
 
+  Context {E} `{impExcE sensitivity_lat -< E, Reg -< E, Memory -< E, IOE sensitivity_lat -< E}.
+
   (** [seq_asm] is denoted as the (horizontal) composition of denotations. *)
   Lemma seq_asm_correct {A B C} (ab : asm A B) (bc : asm B C) :
-      denote_asm (seq_asm ab bc)
+      denote_asm (E := E) (seq_asm ab bc)
     ⩯ denote_asm ab >>> denote_asm bc.
   Proof.
     unfold seq_asm.
@@ -439,23 +441,23 @@ Section Linking.
   Lemma reassoc_seq_asm_exc_B (B C D : nat) (b : fin B) (bc : fin (B + C) ) :
      split_fin_sum B C  bc = inl b -> reassoc_seq_asm_exc (L (D + C) bc) = L (D + C) b.
   Proof.
-    intros. unfold reassoc_seq_asm_exc. cbn.
+    intros HH. unfold reassoc_seq_asm_exc. cbn.
     unfold cat, Cat_sub, cat, Cat_Fun.
     unfold assoc_r, AssocR_Coproduct, case_, Case_sub, case_, Case_Kleisli, case_sum.
     cbn. unfold to_bif, ToBifunctor_Fun_fin. unfold swap, Swap_Coproduct, case_.
-    unfold bimap, Bimap_Coproduct, case_, cat. cbn. rewrite split_fin_sum_L. rewrite H.
+    unfold bimap, Bimap_Coproduct, case_, cat. cbn. rewrite split_fin_sum_L. rewrite HH.
     repeat rewrite split_fin_sum_L. auto.
   Qed.
 
   Lemma reassoc_seq_asm_exc_C_ab (B C D : nat ) (c : fin C) (bc : fin (B + C) ) :
     split_fin_sum B C bc = inr c -> @reassoc_seq_asm_exc B C D (L _ bc ) = R _ (R _ c).
   Proof.
-    intros. unfold reassoc_seq_asm_exc. cbn.
+    intros HH. unfold reassoc_seq_asm_exc. cbn.
     unfold cat, Cat_sub, cat, Cat_Fun.
     unfold assoc_r, AssocR_Coproduct, case_, Case_sub, case_, Case_Kleisli, case_sum.
     cbn. unfold to_bif, ToBifunctor_Fun_fin. unfold swap, Swap_Coproduct, case_.
     unfold bimap, Bimap_Coproduct, case_, cat. cbn.
-    repeat rewrite split_fin_sum_L. repeat rewrite split_fin_sum_R. rewrite H. cbn.
+    repeat rewrite split_fin_sum_L. repeat rewrite split_fin_sum_R. rewrite HH. cbn.
     repeat rewrite split_fin_sum_L. repeat rewrite split_fin_sum_R. cbn.
     repeat rewrite split_fin_sum_L. repeat rewrite split_fin_sum_R. cbn.
     unfold assoc_l, AssocL_Coproduct. cbn. unfold case_.
@@ -468,13 +470,13 @@ Section Linking.
   Lemma reassoc_seq_asm_exc_D (B C D : nat ) (d : fin D) (dc : fin (D + C) ) :
     split_fin_sum D C dc = inl d -> @reassoc_seq_asm_exc B C D (R _ dc ) = R _ (L _ d).
   Proof.
-    intros. unfold reassoc_seq_asm_exc. cbn.
+    intros HH. unfold reassoc_seq_asm_exc. cbn.
     unfold cat, Cat_sub, cat, Cat_Fun.
     unfold assoc_r, AssocR_Coproduct, case_, Case_sub, case_, Case_Kleisli, case_sum.
     cbn. unfold to_bif, ToBifunctor_Fun_fin. unfold swap, Swap_Coproduct, case_.
     unfold bimap, Bimap_Coproduct, case_, cat. cbn.
     repeat rewrite split_fin_sum_L. repeat rewrite split_fin_sum_R. cbn.
-    repeat rewrite split_fin_sum_L. repeat rewrite split_fin_sum_R. cbn. rewrite H.
+    repeat rewrite split_fin_sum_L. repeat rewrite split_fin_sum_R. cbn. rewrite HH.
     unfold assoc_l, AssocL_Coproduct. cbn. unfold case_. cbn.
     repeat rewrite split_fin_sum_L. repeat rewrite split_fin_sum_R. cbn. auto.
   Qed.
@@ -482,12 +484,12 @@ Section Linking.
   Lemma reassoc_seq_asm_exc_C_bd (B C D : nat ) (c : fin C) (dc : fin (D + C) ) :
     split_fin_sum D C dc = inr c -> @reassoc_seq_asm_exc B C D (R _ dc ) = R _ (R _ c).
   Proof.
-    intros. unfold reassoc_seq_asm_exc. cbn.
+    intros HH. unfold reassoc_seq_asm_exc. cbn.
     unfold cat, Cat_sub, cat, Cat_Fun.
     unfold assoc_r, AssocR_Coproduct, case_, Case_sub, case_, Case_Kleisli, case_sum.
     cbn. unfold to_bif, ToBifunctor_Fun_fin. unfold swap, Swap_Coproduct, case_.
     unfold bimap, Bimap_Coproduct, case_, cat. cbn.
-    repeat rewrite split_fin_sum_L. repeat rewrite split_fin_sum_R. cbn. rewrite H.
+    repeat rewrite split_fin_sum_L. repeat rewrite split_fin_sum_R. cbn. rewrite HH.
     repeat rewrite split_fin_sum_L. repeat rewrite split_fin_sum_R. cbn.
     unfold assoc_l, AssocL_Coproduct. cbn. unfold case_. cbn.
     repeat rewrite split_fin_sum_L. repeat rewrite split_fin_sum_R.
@@ -496,14 +498,14 @@ Section Linking.
   Qed.
 
   Lemma seq_asm_exc_correct {A B C D} (ab : asm A (B + C)) (bd : asm B (D + C)) :
-     denote_asm (seq_asm_exc ab bd)
+     denote_asm (E := E) (seq_asm_exc ab bd)
    ⩯ denote_asm ab  >>> case_ (denote_asm bd) inr_.
   Proof.
     unfold seq_asm_exc, expose_linking_labels, swap_and_merge, comb.
     rewrite loop_asm_correct, relabel_asm_correct, app_asm_correct. rewrite cat_id_r.
     repeat rewrite fmap_swap.
     match goal with |- loop ?b ⩯ _ =>  set b as body end.
-    assert (forall a : fin A, body (merge_fin_sum _ _ (inr a)) ≈
+    assert (HH : forall a : fin A, body (merge_fin_sum _ _ (inr a)) ≈
                               r <- denote_asm ab a;;
                          Ret
                            (reassoc_seq_asm_exc (L _ r) )).
@@ -518,7 +520,7 @@ Section Linking.
       unfold from_bif, FromBifunctor_ktree_fin. setoid_rewrite bind_ret_l.
       cbn. unfold unsubm. subst. unfold reassoc_seq_asm_exc. reflexivity.
     } (* this unfolding basically shows that you only need to unfold the top level loop twice*)
-    assert (forall b : fin B, body (merge_fin_sum _ _ (inl b) ) ≈
+    assert (HI : forall b : fin B, body (merge_fin_sum _ _ (inl b) ) ≈
                               r <- denote_asm bd b;;
                          Ret (reassoc_seq_asm_exc (R _ r) )).
     {
@@ -528,16 +530,16 @@ Section Linking.
       unfold from_bif, FromBifunctor_ktree_fin. setoid_rewrite bind_ret_l.
       cbn. unfold unsubm. unfold reassoc_seq_asm_exc. reflexivity.
     }
-    assert (body ⩯ case_
+    assert (HJ : body ⩯ case_
                  (denote_asm bd >>> (fun r => Ret (reassoc_seq_asm_exc (R _ r) ) ))
                  (denote_asm ab >>> (fun r => Ret (reassoc_seq_asm_exc (L _ r)) ))).
     { do 5 red. unfold case_, Case_sub. unfold to_bif, ToBifunctor_ktree_fin.
       cbn.
       intros. destruct (split_fin_sum B A a) eqn : Heq.
-      - rewrite bind_ret_l. cbn. rewrite <- H0. rewrite <- Heq. rewrite merge_split. reflexivity.
-      - rewrite bind_ret_l. cbn. rewrite <- H. rewrite <- Heq. rewrite merge_split. reflexivity.
+      - rewrite bind_ret_l. cbn. rewrite <- HI. rewrite <- Heq. rewrite merge_split. reflexivity.
+      - rewrite bind_ret_l. cbn. rewrite <- HH. rewrite <- Heq. rewrite merge_split. reflexivity.
     }
-    rewrite H1.
+    rewrite HJ.
     do 5 red. intros. Local Opaque denote_asm. unfold loop. cbn.
     rewrite bind_bind. rewrite bind_ret_l. unfold from_bif, FromBifunctor_ktree_fin.
     rewrite bind_ret_l. cbn.
@@ -552,7 +554,7 @@ Section Linking.
       repeat setoid_rewrite bind_ret_l. cbn. rewrite split_fin_sum_L. cbn.
       rewrite bind_bind. setoid_rewrite bind_ret_l. cbn.
       match goal with |- eqit eq true true (ITree.bind _ ?k ) _ => remember k as k_id  end.
-      assert (forall r, k_id r ≈ Ret r ).
+      assert (HK : forall r, k_id r ≈ Ret r ).
       {
         subst. intros. destruct (split_fin_sum _ _ r) as [d | c] eqn : Heqr .
         - erewrite  reassoc_seq_asm_exc_D; eauto. rewrite split_fin_sum_R. cbn.
@@ -572,7 +574,7 @@ Section Linking.
       }
       setoid_rewrite <- bind_ret_r at 3.
       eapply eqit_bind'; try reflexivity. clear Heqk_id. intros; subst.
-      rewrite H2. reflexivity.
+      rewrite HK. reflexivity.
     - erewrite reassoc_seq_asm_exc_C_ab; eauto. rewrite split_fin_sum_R.
       cbn. repeat setoid_rewrite bind_ret_l. rewrite split_merge.
       cbn. unfold from_bif, FromBifunctor_ktree_fin. cbn. reflexivity.
@@ -583,7 +585,7 @@ Section Linking.
   (** [if_asm] is denoted as the ktree first denoting the branching condition,
       then looking-up the appropriate variable and following with either denotation. *)
   Lemma if_asm_correct {A} (e : list instr) (tp fp : asm 1 A) :
-      denote_asm (if_asm e tp fp)
+      denote_asm (E := E) (if_asm e tp fp)
     ⩯ ((fun _ =>
          denote_list e ;;
          v <- trigger (GetReg tmp_if) ;;
@@ -640,7 +642,7 @@ Section Linking.
   Notation label_case := (split_fin_sum _ _).
 
   Lemma while_asm_correct (e : list instr) (p : asm 1 1) :
-      denote_asm (while_asm e p)
+      denote_asm (E := E) (while_asm e p)
     ⩯ (loop (C := sub (ktree _) fin) (fun l : fin (1 + 1) =>
          match label_case l with
          | inl _ =>
@@ -701,7 +703,7 @@ Definition relabel_output  : fin (1 + 2) -> fin (1 + (1 + 2)) :=
 Opaque L.
 
 Lemma while_asm_exc_correct (e : list instr) (p : asm 1 (1 + 2 )) :
-   denote_asm (while_asm_exc e p)
+   denote_asm (E := E) (while_asm_exc e p)
  ⩯ (loop (C := sub (ktree _) fin) (fun l : fin (1 + 1) =>
          match label_case l with
          | inl _ =>
@@ -744,7 +746,7 @@ Proof.
 Qed.
 
 Lemma trycatch_asm_correct (p : asm 1 (1 + (1 + 1) )) (c : asm 1 3) :
-  denote_asm (trycatch_asm p c)
+  denote_asm (E := E) (trycatch_asm p c)
 ⩯ denote_asm p >>> case_ inl_ (merge >>> denote_asm c ).
 Proof.
  unfold trycatch_asm. rewrite seq_asm_correct. repeat rewrite relabel_asm_correct.
@@ -759,24 +761,25 @@ Proof.
  - repeat setoid_rewrite bind_ret_l. cbn. unfold id.
    unfold merge, case_, Case_sub, case_, Case_Kleisli, case_sum, to_bif, ToBifunctor_Fun_fin.
    cbn. setoid_rewrite <- bind_ret_r at 4. eapply eqit_bind' with (RR := eq).
-   + match goal with |- eqit eq true true (denote_asm c ?f1) (denote_asm c (?f2) ) => assert (f1 = f2) end.
+   + match goal with |- eqit eq true true (denote_asm c ?f1) (denote_asm c (?f2) ) => assert (HH : f1 = f2) end.
    { apply unique_fin. auto. }
-   timeout 5 rewrite H. reflexivity.
+   timeout 5 rewrite HH. reflexivity.
    + intros; subst. destruct r2. cbn. apply eqit_Ret. apply unique_fin. cbn. lia.
  - repeat setoid_rewrite bind_ret_l. cbn. setoid_rewrite <- bind_ret_r at 4.
    eapply eqit_bind' with (RR := eq).
-   + match goal with |- eqit eq true true (denote_asm c ?f1) (denote_asm c (?f2) ) => assert (f1 = f2) end.
+   + match goal with |- eqit eq true true (denote_asm c ?f1) (denote_asm c (?f2) ) => assert (HH : f1 = f2) end.
      { apply unique_fin. auto. }
-     rewrite H. reflexivity.
+     rewrite HH. reflexivity.
    + intros; subst. apply eqit_Ret. apply unique_fin. destruct r2. cbn. lia.
 Qed.
 
+  Definition Throw' : Lattice.T -> impExcE sensitivity_lat void := fun e => Throw e.
 
-  Definition link_with_exc : ktree_fin ((impExcE sensitivity_lat) +' Reg +' Memory +' (IOE sensitivity_lat)) (1 + 2) 1  :=
+  Definition link_with_exc : ktree_fin E (1 + 2) 1  :=
     case_ (id_ _)
-    (case_ (C := ktree_fin _ )
-            (fun _ : fin 1 => v <- trigger (Throw Public);; match v : void with end )
-            (fun _ : fin 1 => v <- trigger (Throw Private);; match v : void with end )).
+    (case_ (C := ktree_fin _)
+            (fun _ : fin 1 => v <- trigger (Throw' Public);; match v : void with end )
+            (fun _ : fin 1 => v <- trigger (Throw' Private);; match v : void with end )).
 
   Lemma compile_compile_stmt_correct (s : stmt) :
     denote_asm (compile s)
@@ -784,9 +787,9 @@ Qed.
   Proof.
     unfold compile, link_with_exc.
     cbn in *. rewrite seq_asm_correct. rewrite relabel_asm_correct. remember (app_asm (raise_asm Public) (raise_asm Private) ) as app.
-    assert (denote_asm (app_asm (@id_asm 1) app) ⩯ bimap (denote_asm id_asm) (denote_asm app) ).
+    assert (HH : denote_asm (app_asm (@id_asm 1) app) ⩯ bimap (denote_asm id_asm) (denote_asm (E := E) app)).
     { rewrite app_asm_correct. reflexivity. }
-    rewrite H. unfold id_asm. rewrite pure_asm_correct. rewrite Heqapp.
+    rewrite HH. unfold id_asm. rewrite pure_asm_correct. rewrite Heqapp.
     rewrite app_asm_correct.
     do 5 red. intros. cbn. eapply eqit_bind'; try reflexivity. intros; subst.
     repeat setoid_rewrite bind_bind. repeat setoid_rewrite bind_ret_l. cbn.
@@ -800,7 +803,7 @@ Transparent denote_asm.
       rewrite bind_bind. tau_steps.  apply eqit_Vis. intros [].
   Qed.
 
-  Lemma early_link_with_exc (p1 p2: ktree_fin ((impExcE sensitivity_lat) +' Reg +' Memory +' (IOE sensitivity_lat)) 1 (1 + 2) ) :
+  Lemma early_link_with_exc (p1 p2: ktree_fin E 1 (1 + 2) ) :
     p1 >>> case_ p2 inr_ >>> link_with_exc ⩯ p1 >>> link_with_exc >>> p2 >>> link_with_exc.
   Proof.
     unfold cat, Cat_sub, cat, Cat_Kleisli. cbn. repeat setoid_rewrite bind_bind.
@@ -878,11 +881,12 @@ Section Correctness.
 
    *)
 
+  Notation E1 :=((impExcE sensitivity_lat) +' (IOE sensitivity_lat)).
 
   (*maybe should be strengthened to requiring too state equivalent memories *)
   Definition valid_asm {T} m : Prop := forall (l1 l2 : registers) (g_asm1 g_asm2 : memory),
     Renv g_asm1 g_asm2 ->
-    @eutt ((impExcE sensitivity_lat) +' (IOE sensitivity_lat)) _ _ (state_invariant (@eq T ))
+    eutt (E := E1) (state_invariant (@eq T ))
           (m (l1, g_asm1)) (m (l2, g_asm2)).
 
   Inductive valid_stmt : stmt -> Prop :=
@@ -899,7 +903,7 @@ Section Correctness.
 
   Lemma compile_expr_correct : forall e g_imp g_asm l1 l2 n,
       Renv g_imp g_asm ->
-      eutt (sim_rel l2 n)
+      eutt (E := E1) (sim_rel l2 n)
             (interp_imp_inline (denote_expr e) (l1,g_imp))
             (interp_asm (denote_list (compile_expr n e)) (l2, g_asm) ).
   Proof.
@@ -1137,8 +1141,10 @@ Section Correctness.
              | inr Public => proj1_sig l = 1
              | inr Private => proj1_sig l = 2 end.
 
+  Notation E2 := (Reg +' Memory +' IOE sensitivity_lat).
+
   Lemma throw_prefix_denote_expr (e : expr) :
-     @throw_prefix sensitivity value (Reg +' Memory +' IOE sensitivity_lat) (denote_expr e) ≈ r <- denote_expr e;; Ret (inl r).
+     @throw_prefix sensitivity value E2 (denote_expr e) ≈ r <- denote_expr e;; Ret (inl r).
   Proof.
     induction e.
     - cbn. setoid_rewrite throw_prefix_ev. rewrite bind_trigger.
@@ -1201,16 +1207,15 @@ Section Correctness.
   Lemma exception_to_sum_correct_instr_aux:
     forall i : instr,
       eqit (fun (x : unit + sensitivity) (_ : unit) => x = inl tt) true true
-           (throw_prefix (denote_instr i)) (denote_instr i).
+           (throw_prefix (E := E2) (denote_instr i)) (denote_instr i).
   Proof.
     intros i. destruct i; cbn; repeat setoid_rewrite throw_prefix_bind;
       repeat rewrite bind_bind; try destruct src; cbn; repeat adv; auto.
   Qed.
 
-
-
-  Lemma exception_to_sum_correct (p : asm 1 1) : eutt label_rel (throw_prefix (denote_asm p f0))
-                                                      (denote_asm (exception_to_sum p) f0).
+  Lemma exception_to_sum_correct (p : asm 1 1) :
+     eutt label_rel (throw_prefix (E := E2) (denote_asm p f0))
+       (denote_asm (exception_to_sum p) f0).
   Proof.
     unfold denote_asm. cbn. repeat setoid_rewrite bind_ret_l.  cbn.
     setoid_rewrite throw_prefix_iter. cbn. eapply eutt_iter' with (RI := eq); auto.
@@ -1275,15 +1280,16 @@ Section Correctness.
     - setoid_rewrite (unique_fin _ r1 (fS (fS f0))); auto. reflexivity.
   Qed.
 
-
-  Lemma exception_to_sum_correct_eutt_eq (p : asm 1 1) : eutt eq (throw_prefix (denote_asm p f0))
-                                                      ((denote_asm (exception_to_sum p) f0) >>= (fun x : fin 3 => Ret (fin3tosum x) )).
+  Lemma exception_to_sum_correct_eutt_eq (p : asm 1 1) :
+     eutt eq (throw_prefix (E := E2) (denote_asm p f0))
+       ((denote_asm (exception_to_sum p) f0) >>= (fun x : fin 3 => Ret (fin3tosum x) )).
   Proof.
     apply eutt_label_rel_to_eutt. apply exception_to_sum_correct.
   Qed.
 
-  Lemma exception_to_sum_correct_eutt_eq' (p : asm 1 1) : eutt eq (denote_asm (exception_to_sum p) f0)
-                                                               (throw_prefix (denote_asm p f0) >>= fun x => Ret (sumtofin3 x)).
+  Lemma exception_to_sum_correct_eutt_eq' (p : asm 1 1) :
+    eutt eq (denote_asm (exception_to_sum p) f0)
+      (throw_prefix (E := E2) (denote_asm p f0) >>= fun x => Ret (sumtofin3 x)).
   Proof.
     apply eutt_label_rel_to_eutt'. apply exception_to_sum_correct.
   Qed.
@@ -1314,7 +1320,7 @@ Section Correctness.
       inversion Hs. subst.
       simpl. Opaque denote_asm. cbn.
       assert (denote_asm (seq_asm_exc (compile_stmt s1) (compile_stmt s2)) f0 ≈
-              (denote_asm (compile_stmt s1) >>> case_ (denote_asm (compile_stmt s2)) inr_) f0).
+              (denote_asm (compile_stmt s1) >>> case_ (denote_asm (E := impExcE sensitivity_lat +' E2) (compile_stmt s2)) inr_) f0).
       { specialize (@seq_asm_exc_correct) as Hsaec.
       do 5 red in Hsaec. rewrite Hsaec.  reflexivity. }
       rewrite H. rewrite throw_prefix_bind.
